cut down logrel, progress on the jmp case of ftlr

theories/ftlr/ftlr_base.v
@@ -5,73 +5,43 @@ From cap_machine Require Export logrel.
 
 Section fundamental.
  Context {Σ:gFunctors} {memg:memG Σ} {regg:regG Σ}
-          {stsg : STSG Addr region_type Σ} {heapg : heapG Σ}
-          `{MonRef: MonRefG (leibnizO _) CapR_rtc Σ} {nainv: logrel_na_invs Σ}
+          {nainv: logrel_na_invs Σ}
           `{MachineParameters}.
 
-  Notation STS := (leibnizO (STS_states * STS_rels)).
-  Notation STS_STD := (leibnizO (STS_std_states Addr region_type)).
-  Notation WORLD := (prodO STS_STD STS). 
-  Implicit Types W : WORLD.
-
-  Notation D := (WORLD -n> (leibnizO Word) -n> iProp Σ).
-  Notation R := (WORLD -n> (leibnizO Reg) -n> iProp Σ).
+  Notation D := ((leibnizO Word) -n> iProp Σ).
+  Notation R := ((leibnizO Reg) -n> iProp Σ).
   Implicit Types w : (leibnizO Word).
   Implicit Types interp : (D).
+  
 
-
-  Definition ftlr_instr (W : WORLD) (r : leibnizO Reg) (p p' : Perm)
-        (g : Locality) (b e a : Addr) (w : Word) (i: instr) (ρ : region_type) := 
-      p = RX ∨ p = RWX ∨ (p = RWLX /\ g = Local)
+  Definition ftlr_instr (r : leibnizO Reg) (p : Perm)
+        (b e a : Addr) (w : Word) (i: instr) (P : D) := 
+      p = RX ∨ p = RWX
     → (∀ x : RegName, is_Some (r !! x))
-    → isCorrectPC (inr (p, g, b, e, a))
+    → isCorrectPC (inr (p, b, e, a))
     → (b <= a)%a ∧ (a < e)%a
-    → PermFlows p p'
-    → (if pwl p then region_state_pwl W a else region_state_nwl W a g)
-    → std W !! a = Some ρ
-    → ρ ≠ Revoked ∧ (∀ m, ρ ≠ Static m)
-    → p' ≠ O
     → decodeInstrW w = i
-    -> □ ▷ (∀ a0 a1 a2 a3 a4 a5 a6,
-             full_map a1
-          -∗ (∀ r1 : RegName, ⌜r1 ≠ PC⌝ → ((fixpoint interp1) a0) (a1 !r! r1))
-          -∗ registers_mapsto (<[PC:=inr (a2, a3, a4, a5, a6)]> a1)
-          -∗ region a0
-          -∗ sts_full_world a0
+    -> □ ▷ (∀ a0 a1 a2 a3 a4,
+             full_map a0
+          -∗ (∀ r1 : RegName, ⌜r1 ≠ PC⌝ → (fixpoint interp1) (a0 !r! r1))
+          -∗ registers_mapsto (<[PC:=inr (a1, a2, a3, a4)]> a0)
           -∗ na_own logrel_nais ⊤
-          -∗ ⌜a2 = RX ∨ a2 = RWX ∨ (a2 = RWLX /\ a3 = Local)⌝
-             → □ ([∗ list] a7 ∈ region_addrs a4 a5, ∃ p'0 : Perm, ⌜PermFlows a2 p'0⌝ ∗ read_write_cond a7 p'0 interp                                                                             ∧ ⌜if pwl a2
-                                                                        then region_state_pwl a0 a7
-                                                                        else region_state_nwl a0 a7 a3⌝)
-                 -∗ interp_conf a0)
-    -∗ ([∗ list] a0 ∈ region_addrs b e, ∃ p'0 : Perm,
-                                           ⌜PermFlows p p'0⌝
-                                        ∗ read_write_cond a0 p'0 interp
-                                        ∧ ⌜if pwl p
-                                           then region_state_pwl W a0
-                                           else region_state_nwl W a0 g⌝)
-    -∗ (∀ r1 : RegName, ⌜r1 ≠ PC⌝ → ((fixpoint interp1) W) (r !r! r1))
-    -∗ read_write_cond a p' interp
-    -∗ (▷ if decide (ρ = Temporary ∧ pwl p' = true)
-        then future_pub_mono (λ Wv : WORLD * (leibnizO Word), ((fixpoint interp1) Wv.1) Wv.2) w
-        else future_priv_mono (λ Wv : WORLD * (leibnizO Word), ((fixpoint interp1) Wv.1) Wv.2) w)
-    -∗ ▷ ((fixpoint interp1) W) w
-    -∗ sts_full_world W
+          -∗ ⌜a1 = RX ∨ a1 = RWX⌝
+             → □ (fixpoint interp1) (inr (a1, a2, a3, a4)) -∗ interp_conf)
+    -∗ inv (logN.@a) (∃ w0 : leibnizO Word, a ↦ₐ w0 ∗ P w0)
+    -∗ (∀ r1 : RegName, ⌜r1 ≠ PC⌝ → (fixpoint interp1) (r !r! r1))
+    -∗ ▷ □ (∀ w0 : Word, P w0 -∗ (fixpoint interp1) w0)
     -∗ na_own logrel_nais ⊤
-    -∗ open_region a W
-    -∗ sts_state_std a ρ
-    -∗ a ↦ₐ[p'] w
-    -∗ PC ↦ᵣ inr (p, g, b, e, a)
-    -∗ ([∗ map] k↦y ∈ delete PC (<[PC:=inr (p, g, b, e, a)]> r), k ↦ᵣ y)
+    -∗ a ↦ₐ w
+    -∗ ▷ P w
+    -∗ ▷ ((∃ w0 : leibnizO Word, a ↦ₐ w0 ∗ P w0) ={⊤ ∖ ↑logN.@a,⊤}=∗ emp)
+    -∗ PC ↦ᵣ inr (p, b, e, a)
+    -∗ ([∗ map] k↦y ∈ delete PC (<[PC:=inr (p, b, e, a)]> r), k ↦ᵣ y)
     -∗
         WP Instr Executable
-        {{ v, WP Seq (cap_lang.of_val v)
-                 {{ v0, ⌜v0 = HaltedV⌝
-                        → ∃ (r1 : Reg) (W' : WORLD),
-                        full_map r1
-                        ∧ registers_mapsto r1
-                                           ∗ ⌜related_sts_priv_world W W'⌝
-                                           ∗ na_own logrel_nais ⊤
-                                           ∗ sts_full_world W' ∗ region W' }} }}.
+        @ ⊤ ∖ ↑logN.@a {{ v, |={⊤ ∖ ↑logN.@a,⊤}=> WP Seq (of_val v)
+                                                    {{ v0, ⌜v0 = HaltedV⌝
+                                                           → ∃ r1 : Reg, full_map r1 ∧ registers_mapsto r1
+                                                             ∗ na_own logrel_nais ⊤ }} }}. 
 
 End fundamental.
