theories/logrel.v
@@ -1,7 +1,7 @@
 From iris.proofmode Require Import tactics.
 From iris.program_logic Require Export weakestpre.
 (* From cap_machine.rules Require Export rules. *)
-From cap_machine Require Export cap_lang region region_invariants.
+From cap_machine Require Export cap_lang region.
 From iris.algebra Require Import gmap agree auth.
 From iris.base_logic Require Export invariants na_invariants saved_prop.
 Import uPred.
@@ -31,17 +31,11 @@ Class logrel_na_invs Σ :=
 (** interp : is a unary logical relation. *)
 Section logrel.
   Context {Σ:gFunctors} {memg:memG Σ} {regg:regG Σ}
-          {stsg : STSG Addr region_type Σ} {heapg : heapG Σ}
-          `{MonRef: MonRefG (leibnizO _) CapR_rtc Σ} {nainv: logrel_na_invs Σ}
+          {nainv: logrel_na_invs Σ}
           `{MachineParameters}.
 
-  Notation STS := (leibnizO (STS_states * STS_rels)).
-  Notation STS_STD := (leibnizO (STS_std_states Addr region_type)).
-  Notation WORLD := (prodO STS_STD STS). 
-  Implicit Types W : WORLD.
-
-  Notation D := (WORLD -n> (leibnizO Word) -n> iProp Σ).
-  Notation R := (WORLD -n> (leibnizO Reg) -n> iProp Σ).
+  Notation D := ((leibnizO Word) -n> iProp Σ).
+  Notation R := ((leibnizO Reg) -n> iProp Σ).
   Implicit Types w : (leibnizO Word).
   Implicit Types interp : (D).
 
@@ -53,566 +47,213 @@ Section logrel.
 
   Definition full_map (reg : Reg) : iProp Σ := (∀ (r : RegName), ⌜is_Some (reg !! r)⌝)%I.
   Program Definition interp_reg (interp : D) : R :=
-   λne (W : WORLD) (reg : leibnizO Reg), (full_map reg ∧
-                                          ∀ (r : RegName), (⌜r ≠ PC⌝ → interp W (reg !r! r)))%I.
-  Solve All Obligations with solve_proper.
+   λne (reg : leibnizO Reg), (full_map reg ∧
+                              ∀ (r : RegName), (⌜r ≠ PC⌝ → interp (reg !r! r)))%I.
 
-  Definition interp_conf W : iProp Σ :=
-    (WP Seq (Instr Executable) {{ v, ⌜v = HaltedV⌝ →
-              ∃ r W', full_map r ∧ registers_mapsto r
-                   ∗ ⌜related_sts_priv_world W W'⌝
-                   ∗ na_own logrel_nais ⊤
-                   ∗ sts_full_world W'
-                   ∗ region W' }})%I.
-
+  Definition interp_conf : iProp Σ :=
+    (WP Seq (Instr Executable) {{ v, ⌜v = HaltedV⌝ → ∃ r, full_map r ∧ registers_mapsto r ∗ na_own logrel_nais ⊤ }})%I.
+  
   Program Definition interp_expr (interp : D) r : D :=
-    (λne W w, (interp_reg interp W r ∗ registers_mapsto (<[PC:=w]> r)
-                                     ∗ region W
-                                     ∗ sts_full_world W
-                                     ∗ na_own logrel_nais ⊤ -∗
-                                     ⌜match w with inr _ => True | _ => False end⌝ ∧ interp_conf W))%I.
+    (λne w, (interp_reg interp r ∗ registers_mapsto (<[PC:=w]> r) ∗ na_own logrel_nais ⊤ -∗
+                        ⌜match w with inr _ => True | _ => False end⌝ ∧ interp_conf))%I.
   Solve All Obligations with solve_proper.
-
+  
   (* condition definitions *)
-  Program Definition read_write_cond l p (interp : D) : iProp Σ :=
-    rel l p (λne Wv, interp Wv.1 Wv.2).
-  Next Obligation.
+  Program Definition read_cond (P : D) : D -n> iProp Σ :=
+    λne interp, (▷ □ ∀ (w : Word), P w -∗ interp w)%I.
+  Solve Obligations with solve_proper.
+  Global Instance read_cond_ne n :
+    Proper (dist n ==> dist n ==> dist n) read_cond.
   Proof. solve_proper. Qed.
-  Global Instance read_write_cond_ne n :
-    Proper ((=) ==> (=) ==> dist n ==> dist n) read_write_cond.
-  Proof.
-    rewrite /read_write_cond rel_eq /rel. solve_proper_prepare.
-    f_equiv =>γ. f_equiv.
-    apply saved_anything_ne.
-    solve_proper.
-  Qed.
-
-  Definition future_world g W W' : iProp Σ :=
-    (match g with
-    | Local => ⌜related_sts_pub_world W W'⌝
-    | Global => ⌜related_sts_priv_world W W'⌝
-     end)%I.
-
-  Global Instance future_world_persistent g W W': Persistent (future_world g W W').
-  Proof.
-    unfold future_world. destruct g; apply bi.pure_persistent.
-  Qed.
-
-  Definition exec_cond W b e g p (interp : D) : iProp Σ :=
-    (∀ a r W', ⌜a ∈ₐ [[ b , e ]]⌝ → future_world g W W' →
-            ▷ interp_expr interp r W' (inr ((p,g),b, e,a)))%I.
-  Global Instance exec_cond_ne n :
-    Proper ((=) ==> (=) ==> (=) ==> (=) ==> (=) ==> dist n ==> dist n) exec_cond.
-  Proof. unfold exec_cond. solve_proper. Qed.
-
-  Definition enter_cond W b e a g (interp : D) : iProp Σ :=
-    (∀ r W', future_world g W W' →
-        ▷ interp_expr interp r W' (inr ((RX,g),b,e,a)))%I.
+  
+  Program Definition write_cond (P : D) : D -n> iProp Σ :=
+    λne interp, (▷ □ ∀ (w : Word), interp w -∗ P w)%I.
+  Solve Obligations with solve_proper.
+  Global Instance write_cond_ne n :
+    Proper (dist n ==> dist n ==> dist n) write_cond.
+  Proof. solve_proper. Qed.
+  
+  Program Definition enter_cond b e a : D -n> iProp Σ :=
+    λne interp, (∀ r, ▷ interp_expr interp r (inr (RX,b,e,a)))%I.
+  Solve Obligations with solve_proper.
   Global Instance enter_cond_ne n :
-    Proper ((=) ==> (=) ==> (=) ==> (=) ==> (=) ==> dist n ==> dist n) enter_cond.
-  Proof. unfold enter_cond. solve_proper. Qed.
+    Proper ((=) ==> (=) ==> (=) ==> dist n ==> dist n) enter_cond.
+  Proof. solve_proper. Qed.
 
   (* interp definitions *)
-  Definition interp_z : D := λne _ w, ⌜match w with inl z => True | _ => False end⌝%I.
+  Program Definition interp_ref_inv (a : Addr) : D -n> iProp Σ := λne P, (∃ w, a ↦ₐ w ∗ P w)%I.
+  Solve Obligations with solve_proper.
 
-  Definition interp_cap_O : D := λne _ _, True%I.
+  Definition logN : namespace := nroot .@ "logN".
+  
+  Definition interp_z : D := λne w, ⌜match w with inl z => True | _ => False end⌝%I.
 
-  Definition region_state_pwl W (a : Addr) : Prop :=
-    (std W) !! a = Some Temporary.
-
-  Definition region_state_nwl W (a : Addr) (l : Locality) : Prop :=
-    match l with
-     | Local => (std W) !! a = Some Temporary
-               ∨ (std W) !! a = Some Permanent
-    | Global => (std W) !! a = Some Permanent
-    end.
-
-  Definition region_state_U W (a : Addr) : Prop :=
-    (std W) !! a = Some Temporary
-    \/ (std W) !! a = Some Permanent
-    ∨ (exists w, (std W) !! a = Some (Static {[a:=w]})).
-
-  Definition region_state_U_pwl W (a : Addr) : Prop :=
-    (std W) !! a = Some Temporary
-    ∨ (exists w, (std W) !! a = Some (Static {[a:=w]})).
-
-  (* For simplicity we might want to have the following statement in valididy of caps. However, it is strictly not
-     necessary since it can be derived form full_sts_world *)
-  (* Definition region_std W (a : Addr) : Prop := rel_is_std_i W (countable.encode a). *)
+  Definition interp_cap_O : D := λne _, True%I.
 
   Program Definition interp_cap_RO (interp : D) : D :=
-    λne W w, (match w with
-              | inr ((RO,g),b,e,a) =>
-                [∗ list] a ∈ (region_addrs b e), ∃ p, ⌜PermFlows RO p⌝ ∗ (read_write_cond a p interp) ∧ ⌜region_state_nwl W a g⌝
+    λne w, (match w with
+              | inr (RO,b,e,a) =>
+                [∗ list] a ∈ (region_addrs b e), ∃ P, inv (logN .@ a) (interp_ref_inv a P) ∗ read_cond P interp
               | _ => False
               end)%I.
-  Solve All Obligations with solve_proper.
-     
+  Solve All Obligations with solve_proper.     
 
   Program Definition interp_cap_RW (interp : D) : D :=
-    λne W w, (match w with
-              | inr ((RW,g),b,e,a) =>
-                [∗ list] a ∈ (region_addrs b e), ∃ p, ⌜PermFlows RW p⌝ ∗ (read_write_cond a p interp) ∧ ⌜region_state_nwl W a g⌝
-              | _ => False
-              end)%I.
-  Solve All Obligations with solve_proper.
-
-  Program Definition interp_cap_RWL (interp : D) : D :=
-    λne W w, (match w with
-              | inr ((RWL,Local),b,e,a) =>
-                      [∗ list] a ∈ (region_addrs b e), ∃ p, ⌜PermFlows RWL p⌝ ∗ (read_write_cond a p interp) ∧ ⌜region_state_pwl W a⌝
+    λne w, (match w with
+              | inr (RW,b,e,a) =>
+                [∗ list] a ∈ (region_addrs b e), ∃ P, inv (logN .@ a) (interp_ref_inv a P) ∗ read_cond P interp
+                                                          ∗ write_cond P interp
               | _ => False
               end)%I.
   Solve All Obligations with solve_proper.
 
   Program Definition interp_cap_RX (interp : D) : D :=
-    λne W w, (match w with inr ((RX,g),b,e,a) =>
-                           ([∗ list] a ∈ (region_addrs b e), ∃ p, ⌜PermFlows RX p⌝ ∗ (read_write_cond a p interp)
-                                                                   ∧ ⌜region_state_nwl W a g⌝)
-                                 (* ∗ □ exec_cond W b e g RX interp *)
+    λne w, (match w with inr (RX,b,e,a) =>
+                         [∗ list] a ∈ (region_addrs b e), ∃ P, inv (logN .@ a) (interp_ref_inv a P) ∗ read_cond P interp
              | _ => False end)%I.
   Solve All Obligations with solve_proper.
 
   Program Definition interp_cap_E (interp : D) : D :=
-    λne W w, (match w with
-              | inr ((E,g),b,e,a) => □ enter_cond W b e a g interp
+    λne w, (match w with
+              | inr (E,b,e,a) => □ enter_cond b e a interp
               | _ => False
               end)%I.
   Solve All Obligations with solve_proper.
 
   Program Definition interp_cap_RWX (interp : D) : D :=
-    λne W w, (match w with inr ((RWX,g),b,e,a) =>
-                           ([∗ list] a ∈ (region_addrs b e), ∃ p, ⌜PermFlows RWX p⌝ ∗ (read_write_cond a p interp)
-                                                                   ∧ ⌜region_state_nwl W a g⌝)
-                                 (* ∗ □ exec_cond W b e g RWX interp *)
+    λne w, (match w with inr (RWX,b,e,a) =>
+                           [∗ list] a ∈ (region_addrs b e), ∃ P, inv (logN .@ a) (interp_ref_inv a P) ∗ read_cond P interp
+                                                          ∗ write_cond P interp
              | _ => False end)%I.
   Solve All Obligations with solve_proper.
 
-  Program Definition interp_cap_RWLX (interp : D) : D :=
-    λne W w, (match w with inr ((RWLX,Local),b,e,a) =>
-                           ([∗ list] a ∈ (region_addrs b e), ∃ p, ⌜PermFlows RWLX p⌝ ∗ (read_write_cond a p interp)
-                                                                   ∧ ⌜region_state_pwl W a⌝)
-                                 (* ∗ □ exec_cond W b e Local RWLX interp *)
-             | _ => False end)%I.
-  Solve All Obligations with solve_proper.
-
-  Program Definition interp_cap_URW (interp : D) : D :=
-    λne W w, (match w with
-              | inr ((URW,Local),b,e,a) =>
-                ([∗ list] a' ∈ (region_addrs b (min a e)), ∃ p, ⌜PermFlows (promote_perm URW) p⌝ ∗ (read_write_cond a' p interp)
-                                                                 ∧ ⌜region_state_nwl W a' Local⌝) ∗
-                ([∗ list] a' ∈ (region_addrs (max b a) e), ∃ p, ⌜PermFlows (promote_perm URW) p⌝ ∗ (read_write_cond a' p interp) ∧ ⌜region_state_U W a'⌝)
-              | inr ((URW,Global),b,e,a) =>
-                [∗ list] a' ∈ (region_addrs b e), ∃ p, ⌜PermFlows (promote_perm URW) p⌝ ∗ (read_write_cond a' p interp) ∧ ⌜region_state_nwl W a' Global⌝
-              | _ => False
-              end)%I.
-  Solve All Obligations with solve_proper;auto.
   
-  Program Definition interp_cap_URWL (interp : D) : D :=
-    λne W w, (match w with
-              | inr ((URWL,Local),b,e,a) =>
-                ([∗ list] a' ∈ (region_addrs b (min a e)), ∃ p, ⌜PermFlows (promote_perm URWL) p⌝ ∗ (read_write_cond a' p interp)
-                                                                 ∧ ⌜region_state_pwl W a'⌝) ∗
-                ([∗ list] a' ∈ (region_addrs (max b a) e), ∃ p, ⌜PermFlows (promote_perm URWL) p⌝ ∗ (read_write_cond a' p interp) ∧
-                                                                 ⌜region_state_U_pwl W a'⌝)
-              | _ => False
-              end)%I.
-  Solve All Obligations with solve_proper;auto.
-
-  Program Definition interp_cap_URWX (interp : D) : D :=
-    λne W w, (match w with
-              | inr ((URWX,Local),b,e,a) =>
-                ([∗ list] a' ∈ (region_addrs b (min a e)), ∃ p, ⌜PermFlows (promote_perm URWX) p⌝ ∗ (read_write_cond a' p interp)
-                                                                 ∧ ⌜region_state_nwl W a' Local⌝)
-                      (* ∗ □ exec_cond W b (min a e) Local RWX interp *)
-               ∗ ([∗ list] a' ∈ (region_addrs (max b a) e), ∃ p, ⌜PermFlows (promote_perm URWX) p⌝ ∗ (read_write_cond a' p interp)
-                                                                   ∧ ⌜region_state_U W a'⌝)
-              | inr ((URWX,Global),b,e,a) =>
-                ([∗ list] a' ∈ (region_addrs b e), ∃ p, ⌜PermFlows (promote_perm URWX) p⌝ ∗ (read_write_cond a' p interp)
-                                                                 ∧ ⌜region_state_nwl W a' Global⌝)
-                      (* ∗ □ exec_cond W b e Global RWX interp *)
-             | _ => False end)%I.
-  Solve All Obligations with solve_proper;auto.
-
-  Program Definition interp_cap_URWLX (interp : D) : D :=
-    λne W w, (match w with
-              | inr ((URWLX,Local),b,e,a) =>
-                ([∗ list] a' ∈ (region_addrs b (min a e)), ∃ p, ⌜PermFlows (promote_perm URWLX) p⌝ ∗ (read_write_cond a' p interp)
-                                                                 ∧ ⌜region_state_pwl W a'⌝)
-                      (* ∗ □ exec_cond W b (min a e) Local RWLX interp *)
-                ∗ ([∗ list] a' ∈ (region_addrs (max b a) e), ∃ p, ⌜PermFlows (promote_perm URWLX) p⌝ ∗ (read_write_cond a' p interp) ∧
-                                                                   ⌜region_state_U_pwl W a'⌝)
-             | _ => False end)%I.
-  Solve All Obligations with solve_proper;auto.
-
   Program Definition interp1 (interp : D) : D :=
-    (λne W w,
+    (λne w,
     match w return _ with
-    | inl _ => interp_z W w
-    | inr ((O, g), b, e, a) => interp_cap_O W w
-    | inr ((RO, g), b, e, a) => interp_cap_RO interp W w
-    | inr ((RW, g), b, e, a) => interp_cap_RW interp W w
-    | inr ((RWL, g), b, e, a) => interp_cap_RWL interp W w
-    | inr ((RX, g), b, e, a) => interp_cap_RX interp W w
-    | inr ((E, g), b, e, a) => interp_cap_E interp W w
-    | inr ((RWLX, g), b, e, a) => interp_cap_RWLX interp W w
-    | inr ((RWX, g), b, e, a) => interp_cap_RWX interp W w
-    | inr ((URW, g), b, e, a) => interp_cap_URW interp W w
-    | inr ((URWL, g), b, e, a) => interp_cap_URWL interp W w
-    | inr ((URWLX, g), b, e, a) => interp_cap_URWLX interp W w
-    | inr ((URWX, g), b, e, a) => interp_cap_URWX interp W w
+    | inl _ => interp_z w
+    | inr (O, b, e, a) => interp_cap_O w
+    | inr (RO, b, e, a) => interp_cap_RO interp w
+    | inr (RW, b, e, a) => interp_cap_RW interp w
+    | inr (RX, b, e, a) => interp_cap_RX interp w
+    | inr (E, b, e, a) => interp_cap_E interp w
+    | inr (RWX, b, e, a) => interp_cap_RWX interp w
     end)%I.
-  Solve All Obligations with solve_proper.
 
-  (* Global Instance interp_expr_contractive : *)
-  (*   Contractive (interp_expr). *)
-  (* Proof. solve_contractive. Qed.  *)
+  
+  Global Instance read_cond_contractive :
+    Contractive (read_cond).
+  Proof. solve_contractive. Qed.
   Global Instance interp_cap_O_contractive :
     Contractive (interp_cap_O).
   Proof. solve_contractive. Qed.
   Global Instance interp_cap_RO_contractive :
     Contractive (interp_cap_RO).
-  Proof. solve_proper_prepare.
-         destruct x1; auto. destruct c, p, p, p, p; auto.
-         apply big_opL_ne; auto. rewrite /pointwise_relation; intros.
-         apply exist_ne. rewrite /pointwise_relation; intros.
-         apply sep_ne; auto.
-         rewrite /read_write_cond rel_eq /rel_def /saved_pred_own.
-         apply and_ne; auto.
-         apply exist_ne =>γ. apply sep_ne; auto.
-         simpl. f_equiv. solve_contractive.
-  Qed.
+  Proof.
+    solve_proper_prepare.
+    destruct x0; auto. destruct c, p, p, p; auto.
+    solve_contractive. 
+  Qed.   
   Global Instance interp_cap_RW_contractive :
     Contractive (interp_cap_RW).
-  Proof. solve_proper_prepare. destruct x1; auto. destruct c, p, p, p, p; auto.
-         apply big_opL_ne; auto. rewrite /pointwise_relation; intros.
-         apply exist_ne. rewrite /pointwise_relation; intros.
-         apply sep_ne; auto.
-         rewrite /read_write_cond rel_eq /rel_def /saved_pred_own.
-         apply and_ne;auto. apply exist_ne =>γ. apply sep_ne; auto.
-         simpl. f_equiv. solve_contractive.
-  Qed.
-  Global Instance interp_cap_RWL_contractive :
-    Contractive (interp_cap_RWL).
-  Proof. solve_proper_prepare.
-         destruct x1; auto. destruct c, p, p, p, p, l; auto.
-         apply big_opL_ne; auto. rewrite /pointwise_relation; intros.
-         apply exist_ne. rewrite /pointwise_relation; intros.
-         apply sep_ne; auto.
-         rewrite /read_write_cond rel_eq /rel_def /saved_pred_own.
-         apply and_ne;auto. apply exist_ne =>γ. apply sep_ne; auto.
-         simpl. f_equiv. solve_contractive.
-  Qed.
-  Global Instance exec_cond_contractive W b e g pl :
-    Contractive (λ interp, exec_cond W b e g pl interp).
   Proof.
-    solve_contractive.
+    solve_proper_prepare.
+    destruct x0; auto. destruct c, p, p, p; auto.     
+    solve_contractive. 
   Qed.
-  Global Instance enter_cond_contractive W b e a g :
-    Contractive (λ interp, enter_cond W b e a g interp).
+  Global Instance enter_cond_contractive b e a :
+    Contractive (λ interp, enter_cond b e a interp).
   Proof.
     solve_contractive.
   Qed.
   Global Instance interp_cap_RX_contractive :
     Contractive (interp_cap_RX).
   Proof.
-    rewrite /interp_cap_RX.
     solve_proper_prepare.
-    destruct x1; auto. destruct c, p, p, p, p; auto.
-    - rewrite /read_write_cond rel_eq /rel_def /saved_pred_own.
-      apply big_opL_ne; auto. intros ? ?.
-      apply exist_ne. rewrite /pointwise_relation; intros.
-      apply sep_ne; auto. (* apply sep_ne; auto. *)
-      apply and_ne;auto. apply exist_ne =>γ. apply sep_ne; auto.
-      simpl. f_equiv. solve_contractive.
-    (* - solve_proper_prepare. *)
-    (*   by apply affinely_ne; apply persistently_ne; apply exec_cond_contractive. *)
+    destruct x0; auto. destruct c, p, p, p; auto.
+    solve_contractive. 
   Qed.
   Global Instance interp_cap_E_contractive :
     Contractive (interp_cap_E).
   Proof.
-    rewrite /interp_cap_E.
     solve_proper_prepare.
-    destruct x1; auto. destruct c, p, p, p, p; auto.
-    solve_proper_prepare.
-      by apply affinely_ne; apply persistently_ne; apply enter_cond_contractive.
+    destruct x0; auto. destruct c, p, p, p; auto.
+    solve_contractive. 
   Qed.
   Global Instance interp_cap_RWX_contractive :
     Contractive (interp_cap_RWX).
   Proof.
-    rewrite /interp_cap_RWX. 
     solve_proper_prepare.
-    destruct x1; auto. destruct c, p, p, p, p; auto.
-    - rewrite /read_write_cond rel_eq /rel_def /saved_pred_own.
-      apply big_opL_ne; auto. intros ? ?.
-      apply exist_ne. rewrite /pointwise_relation; intros.
-      apply sep_ne; auto. (* apply sep_ne. *)
-      apply and_ne;auto. apply exist_ne =>γ. apply sep_ne; auto.
-      simpl. f_equiv. solve_contractive.
-    (* - solve_proper_prepare. *)
-    (*   by apply affinely_ne; apply persistently_ne; apply exec_cond_contractive. *)
+    destruct x0; auto. destruct c, p, p, p; auto.
+    solve_contractive. 
   Qed.
-  Global Instance interp_cap_RWLX_contractive :
-    Contractive (interp_cap_RWLX).
-  Proof.
-    rewrite /interp_cap_RWLX.
-    solve_proper_prepare.
-    destruct x1; auto. destruct c, p, p, p, p, l; auto.
-    - rewrite /read_write_cond rel_eq /rel_def /saved_pred_own.
-      apply big_opL_ne; auto. intros ? ?.
-      apply exist_ne. rewrite /pointwise_relation; intros.
-      apply sep_ne; auto. (* apply sep_ne. *)
-      apply and_ne;auto. apply exist_ne =>γ. apply sep_ne; auto.
-      simpl. f_equiv. solve_contractive.
-    (* - solve_proper_prepare. *)
-    (*   by apply affinely_ne; apply persistently_ne; apply exec_cond_contractive. *)
-  Qed.
-  Global Instance interp_cap_URW_contractive :
-    Contractive (interp_cap_URW).
-  Proof. solve_proper_prepare. destruct x1; auto. destruct_cap c; destruct c; destruct c3; auto.
-         - apply big_opL_ne; auto. rewrite /pointwise_relation; intros.
-           apply exist_ne. rewrite /pointwise_relation; intros.
-           apply sep_ne; auto.
-           rewrite /read_write_cond rel_eq /rel_def /saved_pred_own.
-           apply and_ne;auto. apply exist_ne =>γ. apply sep_ne; auto.
-           simpl. f_equiv. solve_contractive.
-         - apply sep_ne; auto.
-           apply big_opL_ne; auto; rewrite /pointwise_relation; intros.
-           apply exist_ne. rewrite /pointwise_relation; intros.
-           apply sep_ne; auto.
-           rewrite /read_write_cond rel_eq /rel_def /saved_pred_own.
-           apply and_ne;auto. apply exist_ne =>γ. apply sep_ne; auto.
-           simpl. f_equiv. solve_contractive.
-           apply big_opL_ne; auto. rewrite /pointwise_relation; intros.
-           rewrite /read_write_cond rel_eq /rel_def /saved_pred_own.
-           apply exist_ne. rewrite /pointwise_relation; intros.
-           apply sep_ne; auto.
-           apply and_ne; auto. apply exist_ne => γ. apply sep_ne; auto.
-           simpl. f_equiv. solve_contractive.
-  Qed.
-  Global Instance interp_cap_URWL_contractive :
-    Contractive (interp_cap_URWL).
-  Proof. solve_proper_prepare.
-         destruct x1; auto. destruct_cap c. destruct c; auto. destruct c3; auto.
-         apply sep_ne; auto.
-         apply big_opL_ne; auto. rewrite /pointwise_relation; intros.
-         apply exist_ne. rewrite /pointwise_relation; intros.
-         apply sep_ne; auto. rewrite /read_write_cond rel_eq /rel_def /saved_pred_own.
-         apply and_ne;auto. apply exist_ne =>γ. apply sep_ne; auto.
-         simpl. f_equiv. solve_contractive.
-         apply big_opL_ne; auto. rewrite /pointwise_relation; intros.
-         rewrite /read_write_cond rel_eq /rel_def /saved_pred_own.
-         apply exist_ne. rewrite /pointwise_relation; intros.
-         apply sep_ne; auto. 
-         apply and_ne; auto. apply exist_ne => γ. apply sep_ne; auto.
-         simpl. f_equiv. solve_contractive.
-  Qed.
-  Global Instance interp_cap_URWX_contractive :
-    Contractive (interp_cap_URWX).
-  Proof.
-    rewrite /interp_cap_URWX.
-    solve_proper_prepare.
-    destruct x1; auto. destruct_cap c; destruct c; destruct c3; auto.
-    - rewrite /read_write_cond rel_eq /rel_def /saved_pred_own.
-      apply big_opL_ne; auto. intros ? ?.
-      apply exist_ne. rewrite /pointwise_relation; intros.
-      apply sep_ne; auto.
-      apply and_ne;auto. apply exist_ne =>γ. apply sep_ne; auto.
-      simpl. f_equiv. solve_contractive.
-    - apply sep_ne; auto.
-      + apply big_opL_ne; auto. rewrite /pointwise_relation; intros.
-        apply exist_ne. rewrite /pointwise_relation; intros.
-        apply sep_ne; auto.
-        rewrite /read_write_cond rel_eq /rel_def /saved_pred_own.
-        apply and_ne; auto. apply exist_ne =>γ. apply sep_ne; auto.
-        simpl. f_equiv. solve_contractive.
-      + apply big_opL_ne; auto. rewrite /pointwise_relation; intros.
-        apply exist_ne. rewrite /pointwise_relation; intros.
-        apply sep_ne; auto. 
-        rewrite /read_write_cond rel_eq /rel_def /saved_pred_own.
-        apply and_ne; auto. apply exist_ne => γ. apply sep_ne; auto.
-        simpl. f_equiv. solve_contractive.
-  Qed.
-  Global Instance interp_cap_URWLX_contractive :
-    Contractive (interp_cap_URWLX).
-  Proof.
-    rewrite /interp_cap_URWLX.
-    solve_proper_prepare.
-    destruct x1; auto. destruct_cap c; destruct c; auto. destruct c3; auto.
-    apply sep_ne.
-    - rewrite /read_write_cond rel_eq /rel_def /saved_pred_own.
-      apply big_opL_ne; auto. intros ? ?.
-      apply exist_ne. rewrite /pointwise_relation; intros.
-      apply sep_ne; auto. 
-      apply and_ne;auto. apply exist_ne =>γ. apply sep_ne; auto.
-      simpl. f_equiv. solve_contractive.
-    - apply big_opL_ne; auto. rewrite /pointwise_relation; intros.
-      apply exist_ne. rewrite /pointwise_relation; intros.
-      apply sep_ne; auto. 
-      rewrite /read_write_cond rel_eq /rel_def /saved_pred_own.
-      apply and_ne; auto. apply exist_ne => γ. apply sep_ne; auto.
-      simpl. f_equiv. solve_contractive.
-  Qed.
+  
 
   Global Instance interp1_contractive :
     Contractive (interp1).
   Proof.
-    intros n x y Hdistn W w.
+    intros n x y Hdistn w.
     rewrite /interp1.
     destruct w; [auto|].
-    destruct c,p,p,p,p; first auto.
+    destruct c,p,p,p; first auto.
     - by apply interp_cap_RO_contractive.
     - by apply interp_cap_RW_contractive.
-    - by apply interp_cap_RWL_contractive.
     - by apply interp_cap_RX_contractive.
     - by apply interp_cap_E_contractive.
     - by apply interp_cap_RWX_contractive.
-    - by apply interp_cap_RWLX_contractive.
-    - by apply interp_cap_URW_contractive.
-    - by apply interp_cap_URWL_contractive.
-    - by apply interp_cap_URWX_contractive.
-    - by apply interp_cap_URWLX_contractive.
   Qed.
 
-  Lemma fixpoint_interp1_eq (W : WORLD) (x : leibnizO Word) :
-    fixpoint (interp1) W x ≡ interp1 (fixpoint (interp1)) W x.
-  Proof. exact: (fixpoint_unfold (interp1) W x). Qed.
+  Lemma fixpoint_interp1_eq (x : leibnizO Word) :
+    fixpoint (interp1) x ≡ interp1 (fixpoint (interp1)) x.
+  Proof. exact: (fixpoint_unfold (interp1) x). Qed.
 
-  Program Definition interp : D :=
-    λne W w, (fixpoint (interp1)) W w.
-  Solve All Obligations with solve_proper.
+  Definition interp : D := λne w, (fixpoint (interp1)) w.
   Definition interp_expression r : D := interp_expr interp r.
   Definition interp_registers : R := interp_reg interp.
 
-  Global Instance interp_persistent : Persistent (interp W w).
+  Global Instance interp_persistent : Persistent (interp w).
   Proof. intros. destruct w; simpl; rewrite fixpoint_interp1_eq; simpl.
-         apply _.
-         destruct c,p,p,p,p; destruct l; repeat (apply exist_persistent; intros); try apply _.
+         apply _. destruct c,p,p,p; repeat (apply exist_persistent; intros); try apply _.
   Qed.
-
-  Instance ne_interpC : NonExpansive
-                           (λ Wv : (WORLD * (leibnizO Word)), (interp Wv.1) Wv.2).
-  Proof. intros. solve_proper. Qed.
-
-  (* Non-curried version of interp *)
-  Definition interpC :=
-    (λne Wv : WORLD * (leibnizO Word), (interp Wv.1) Wv.2).
-
-  Lemma read_allowed_inv W (a' a b e: Addr) p g :
+  
+  Lemma read_allowed_inv (a' a b e: Addr) p :
     (b ≤ a' ∧ a' < e)%Z →
-    readAllowed p → (interp W (inr ((p,g),b,e,a)) →
-      (∃ p', ⌜PermFlows p p'⌝ ∗ (read_write_cond a' p' interp)))%I.
+    readAllowed p →
+    (interp (inr (p,b,e,a)) →
+     (∃ P, inv (logN .@ a') (interp_ref_inv a' P) ∗ read_cond P interp))%I.
   Proof.
     iIntros (Hin Ra) "Hinterp".
     rewrite /interp. cbn. rewrite fixpoint_interp1_eq /=; cbn.
-    destruct p,g; try contradiction;
+    destruct p; try contradiction;
     try (iDestruct "Hinterp" as "[Hinterp Hinterpe]");
-    try (iDestruct (extract_from_region_inv with "Hinterp") as (p Hflows) "[Hinv _]"; [eauto|iExists _;iSplit;eauto]).
-    - done.
-    - done.
+    try (iDestruct (extract_from_region_inv with "Hinterp") as (P) "[Hinv Hiff]"; [eauto|iExists P;iSplit;eauto]).
+    - iDestruct "Hiff" as "[Hread Hwrite]". iFrame. 
+    - iDestruct "Hiff" as "[Hread Hwrite]". iFrame. 
+  Qed.
+
+  Lemma write_allowed_inv (a' a b e: Addr) p :
+    (b ≤ a' ∧ a' < e)%Z →
+    writeAllowed p →
+    (interp (inr (p,b,e,a)) →
+     inv (logN .@ a') (interp_ref_inv a' interp))%I.
+  Proof.
+    iIntros (Hin Wa) "Hinterp".
+    rewrite /interp. cbn. rewrite fixpoint_interp1_eq /=; cbn.
+    destruct p; try contradiction.
+    - iDestruct (extract_from_region_inv with "Hinterp") as (P) "[Hinv #[Hread Hwrite] ]";[eauto|].
+      iApply (inv_iff with "[] Hinv"). 
+      iNext. iAlways. iSplit.
+      + iIntros "HP". iDestruct "HP" as (w) "[Ha' HP]".
+        iExists w. iFrame. iApply "Hread". iFrame.
+      + iIntros "HP". iDestruct "HP" as (w) "[Ha' HP]".
+        iExists w. iFrame. iApply "Hwrite". iFrame.
+    - iDestruct (extract_from_region_inv with "Hinterp") as (P) "[Hinv #[Hread Hwrite] ]";[eauto|].
+      iApply (inv_iff with "[] Hinv"). 
+      iNext. iAlways. iSplit.
+      + iIntros "HP". iDestruct "HP" as (w) "[Ha' HP]".
+        iExists w. iFrame. iApply "Hread". iFrame.
+      + iIntros "HP". iDestruct "HP" as (w) "[Ha' HP]".
+        iExists w. iFrame. iApply "Hwrite". iFrame.
   Qed.
   
-  Lemma writeLocalAllowed_implies_local W p l b e a:
-    pwl p = true ->
-    interp W (inr (p, l, b, e, a)) -∗ ⌜isLocal l = true⌝.
-  Proof.
-    intros. iIntros "Hvalid".
-    unfold interp; rewrite fixpoint_interp1_eq /=.
-    destruct p; simpl in H; try congruence; destruct l; eauto.
-  Qed.
-
-  Lemma readAllowed_valid_cap_implies W p l b e a:
-    readAllowed p = true ->
-    withinBounds (p, l, b, e, a) = true ->
-    interp W (inr (p, l, b, e, a)) -∗
-           ⌜∃ ρ, std W !! a = Some ρ ∧ ρ <> Revoked ∧ (∀ g, ρ ≠ Static g)⌝.
-  Proof.
-    intros Hp Hb. iIntros "H".
-    eapply withinBounds_le_addr in Hb.
-    unfold interp; rewrite fixpoint_interp1_eq /=.
-    destruct p; simpl in Hp; try congruence.
-    - iDestruct (extract_from_region_inv with "H") as (p ?) "[_ H]"; eauto.
-      iDestruct "H" as %HH. iPureIntro. destruct l; eauto. simpl in HH.
-      destruct HH; eauto.
-    - iDestruct (extract_from_region_inv with "H") as (p ?) "[_ H]"; eauto.
-      iDestruct "H" as %HH. iPureIntro. destruct l; eauto. simpl in HH.
-      destruct HH; eauto.
-    - destruct l; auto.
-      iDestruct (extract_from_region_inv with "H") as (p ?) "[_ %]"; eauto.
-    - iDestruct (extract_from_region_inv with "H") as (p ?) "[_ H]"; eauto.
-      iDestruct "H" as %HH. iPureIntro. destruct l; eauto. simpl in HH.
-      destruct HH; eauto.
-    - iDestruct (extract_from_region_inv with "H") as (p ?) "[_ H]"; eauto.
-      iDestruct "H" as %HH. iPureIntro. destruct l; eauto. simpl in HH.
-      destruct HH; eauto.
-    - destruct l;auto.
-      iDestruct (extract_from_region_inv with "H") as (p ?) "[_ %]"; eauto.
-  Qed.
-
-  Definition region_conditions W p g b e:=
-  ([∗ list] a ∈ (region_addrs b e), ∃ p', ⌜PermFlows p p'⌝ ∗ (read_write_cond a p' interp)
-                                             ∧ ⌜if pwl p then region_state_pwl W a else region_state_nwl W a g⌝)%I.
-
-  Lemma readAllowed_implies_region_conditions W p l b e a:
-    readAllowed p = true ->
-    interp W (inr (p, l, b, e, a)) -∗ region_conditions W p l b e.
-  Proof.
-    intros. iIntros "Hvalid".
-    unfold interp; rewrite fixpoint_interp1_eq /=.
-    unfold region_conditions.
-    destruct p; simpl in *; try congruence; destruct l; simpl; auto.
-  Qed.
-
-
-  Lemma writeLocalAllowed_valid_cap_implies W p l b e a:
-    pwl p = true ->
-    withinBounds (p, l, b, e, a) = true ->
-    interp W (inr (p, l, b, e, a)) -∗
-           ⌜std W !! a = Some Temporary⌝.
-  Proof.
-    intros Hp Hb. iIntros "Hvalid".
-    iAssert (⌜isLocal l = true⌝)%I as "%". by iApply writeLocalAllowed_implies_local.
-    eapply withinBounds_le_addr in Hb.
-    unfold interp; rewrite fixpoint_interp1_eq /=.
-    destruct p; simpl in Hp; try congruence; destruct l.
-    - by exfalso.
-    - iDestruct (extract_from_region_inv with "Hvalid") as (? ?) "[_ %]"; eauto.
-    - by exfalso.
-    - iDestruct (extract_from_region_inv with "Hvalid") as (? ?) "[_ %]"; eauto.
-  Qed.
-
-  Lemma interp1_eq interp (W: WORLD) p l b e a:
-    ((interp1 interp W (inr (p, l, b, e, a))) ≡
-             (if perm_eq_dec p O then True else
-             if perm_eq_dec p E then □ enter_cond W b e a l interp else
-               ([∗ list] a ∈ region_addrs b (if isU p && isLocal l then (min a e) else e),
-                ∃ p', ⌜PermFlows (promote_perm p) p'⌝ ∗
-                 (read_write_cond a p' interp) ∧
-                 ⌜if pwlU p then region_state_pwl W a else region_state_nwl W a l⌝) ∗
-                (*(□ match p with RX | RWX | RWLX => exec_cond W b e l p interp | URWX | URWLX => exec_cond W b (if isLocal l then min a e else e) l (promote_perm p) interp | _ => True end) ∗*)
-                (⌜if pwlU p then l = Local else True⌝) ∗
-                (if isU p && isLocal l then [∗ list] a ∈ region_addrs (max b a) e,
-                                            ∃ p', ⌜PermFlows (promote_perm p) p'⌝ ∗ read_write_cond a p' interp ∧ ⌜if pwlU p then region_state_U_pwl W a else region_state_U W a⌝ else emp%I))%I).
-  Proof.
-    iSplit.
-    { iIntros "HA".
-      destruct (perm_eq_dec p O); subst; simpl; auto.
-      destruct (perm_eq_dec p E); subst; simpl; auto.
-      destruct p; simpl; try congruence; auto; destruct l;auto. 
-      - iDestruct "HA" as "[HA HB]"; eauto.
-      - iDestruct "HA" as "[HA HB]"; eauto.
-      - iDestruct "HA" as "[Ha HB]"; eauto.
-      - iDestruct "HA" as "[HB HC]"; eauto. }
-    { iIntros "A".
-      destruct (perm_eq_dec p O); subst; simpl; auto.
-      destruct (perm_eq_dec p E); subst; simpl; auto.
-      iDestruct "A" as "(B & % & C)".
-      destruct p; simpl in *; try congruence; subst; eauto; destruct l; eauto. }
-  Qed.
-
 End logrel.
-
-(* Notation "𝕍( W )" := (interp W) (at level 70). *)
-(* Notation "𝔼( W )" := (λ r, interp_expression r W). *)
-(* Notation "ℝ( W )" := (interp_registers W). *)
-(* Notation "𝕆( W )" := (interp_conf W.1 W.2).  *)
